%!TEX root = ../AppendixC.tex
\section{Sample Complexity of \texorpdfstring{\LG{}}{}}\label{app:lgc.proof}

\subsection{Events}\label{app:lgc.proof_nc.events}
We fix a constant $\alpha>2$ and define the event
\[
\cE_t = \left\{\forall s \leq  t:\ \frac{1}{2}\normm{\hbtheta_s-\btheta}^2_{\bLambda_{T_s}+\lambda I_d} \leq h(t)\eqdef d_{t,1/t^\alpha}\right\}\,.
\]
This event holds with high probability
\begin{lemma}
\label{lem:prb_Et_nc}
For all $t \geq 1$
\[
    \PPt{\left(\cE_t^c\right)}\leq \frac{1}{t^{\alpha-1}}\,.
\]
\end{lemma}
We now prove that we can construct, on this event, upper confidence bounds on the loss given to the learners.
\begin{lemma}
\label{lem:confidence_bound_general_nc}
On the event $\cE_t$, for all $(\bx,i)\in\cX\times\cI$ and $\btheta'\in\neg i$, for all $s\leq t$,
\[
\normm{\btheta-\btheta'}^2_{\bx\bx\transpose} \leq \min\left(\max_\pm \left( \langle \hbtheta_{s} - \btheta',\bx\rangle \pm \sqrt{2 h(t)} \normm{\bx}_{(\bLambda_{T_s}+ \lambda I_d)^{-1}} \right)^2,4M^2\right)
\]
\end{lemma}
\begin{proof}
First, note that since $\btheta,\btheta'\in\cM$, their norms are bounded by $M$, thus it holds
\[
\normm{\btheta-\btheta'}^2_{\bx\bx\transpose} = \langle\btheta-\btheta',\bx \rangle^2 \leq \normm{\btheta-\btheta'}^2 \normm{\btheta'}^2 \leq 4M^2L^2\,.
\]
Furthermore on $\cE_t$ we have
\begin{align*}
\normm{\btheta-\btheta'}^2_{\bx\bx\transpose} = \langle\btheta-\btheta',\bx \rangle^2 &\leq \sup_{\big\{\btheta':\ \normm{\hbtheta_s-\btheta'}^2_{(\bLambda_{T_s} + \lambda I_d)^{-1} } \leq 2h(t)\big\}} \langle\btheta'-\btheta',\bx \rangle^2\\
&=\max_\pm \left( \langle \hbtheta_{s} - \btheta',\bx\rangle \pm \sqrt{2 h(t)} \normm{\bx}_{(\bLambda_{T_s}+ \lambda I_d)^{-1}} \right)^2\,.
\end{align*}
Combining the two inequalities above allows us to conclude.
\end{proof}
We thus define the upper confidence $U_s^{\bx,i}$ on the coordinate $(\bx,i)$ of the loss at time $s\leq t$,
\begin{equation}
\label{eq:def_ucb_br_general_nc}
U_s^{\bx,i} = \min\left(\max_\pm \left( \langle \hbtheta_{s-1} - \btheta',\bx\rangle \pm \sqrt{2 h(t)} \normm{\bx}_{(\bLambda_{\bT_{s-1}}+ \lambda I_d)^{-1}} \right)^2,4M^2\right)\,.
\end{equation}
The first step of our analysis is to restrict it to the event $\mathcal E_t$, as is done by \citet{garivier2016tracknstop,degenne2019game}.
\begin{lemma}
Let $\mathcal E_t$ be an event and $T_0(\delta) \in \NN$ be such that for $t\ge T_0(\delta)$, $\mathcal E_t \subseteq \{\tau_\delta \le t\}$. Then
\begin{align*}
\mathbb{E}[\tau_\delta]
&\le T_0(\delta) + \sum_{t=T_0(\delta)}^{+\infty} \mathbb{P}(\mathcal E_T^c)
\\
&\le T_0(\delta) + \sum_{t=1}^{+\infty} \frac{1}{t^{\alpha-1}}\: .
\end{align*}
\end{lemma}

We need to prove that if $\mathcal E_t$ holds, there exists such a time $T_0(\delta)$.

\subsection{Analysis under concentration}
%\todo[inline]{ We prove that $d_{t,\delta} \geq T_{t,\istar} \Tstar(\btheta)^{-1}$ and that $T_{t,i} = O(\sqrt{t})$ ,for all $i\neq \istar$}
In this section we assume that the event $\cE_t$ holds. And we set $\istar=\Istar(\btheta)$ and define the following quantities
\[
w_t^i = \ind_{\{i_t = i\}}w_t \quad W_t^i = \sum_{s=1}^t w_s^i\quad T_{t,i} = \sum_{s=1}^t \ind{\{\hbx_t=\bx,i_t=i\}}\,.
\]
%That algorithm starts stage $t$ by setting $i_t = i^*(\hbtheta_t)$.

\subsection{When $i_s = \istar$.}
If the algorithm does not stop at stage $t$
%, then let $i_t = i^*(\hat{\btheta}_t$. We have
we have
\begin{align*}
d_{t,\delta}
\ge \frac{1}{2}\max_{i\in\cI} \inf_{\btheta'_i \in \neg i}\Vert \hat{\btheta}_t - \btheta'_i \Vert_{\bLambda_{\bT_t}}^2
\geq  \frac{1}{2} \inf_{\btheta' \in \neg \istar(\btheta)}\Vert \hat{\btheta}_t - \btheta' \Vert_{\bLambda_{\bT_t}}^2
%\ge \frac{1}{2}\sum_{i\in\cI} \inf_{\btheta'_i \in \neg i}\Vert \hat{\btheta}_t - \btheta'_i \Vert_{\bLambda_{T_{t,i}}}^2
\: ,
\end{align*}
Let $\btheta'_{i,w}(\btheta) \in \argmin_{\btheta' \in \neg i} \Vert \btheta - \btheta' \Vert_{\bLambda_{w}}$ , such that we have $d_{t,\delta} \ge \frac{1}{2}\Vert \hat{\btheta}_t - \btheta'_{\istar,\bT_t}(\hat{\btheta}_t) \Vert_{\bLambda_{\bT_t}}^2$ . We first transform that norm into a sum over the rounds of divergences from $\hat{\btheta}_{s-1}$ (instead of $\hat{\btheta}_t$).

\begin{lemma}\label{lem:nc_proof_to_online_formulation}
If $\mathcal E_t$ holds, then an algorithm using C-Tracking ensures that
\begin{align*}
    &\frac{1}{2}\Vert \hat{\btheta}_t - \btheta'_{\istar,\bT_t}(\hat{\btheta}_t) \Vert_{\bLambda_{\bT_t}}^2 + 20 A\left(\sqrt{h(t)g(t) \frac{1}{2}\Vert \hat{\btheta}_t - \btheta'_{\istar,\bT_t}(\hat{\btheta}_t) \Vert_{\bLambda_{\bT_t}}^2}+ 2h(t)g(t)\right)\\
    &\geq \frac{1}{2}\sum_{s=1}^t \Vert \hat{\btheta}_{s-1} - \btheta'_{\istar,\bT_t}(\hat{\btheta}_t)\Vert_{\bLambda_{\tw_s}}^2\,.
\end{align*}
\end{lemma}
\begin{proof}

Using the triangular inequality,
\begin{align*}
\Vert \btheta - \hat{\btheta}_t \Vert_{\bLambda_{\bT_t}} + \Vert \hat{\btheta}_t - \btheta'_{\istar,\bT_t}(\hbtheta_t) \Vert_{\bLambda_{\bT_t}}
\ge \Vert \btheta - \btheta'_{\istar,T_t}(\hat{\btheta}_t) \Vert_{\bLambda_{\bT_t}}
%\ge \Vert \btheta - \btheta'_{i,T_{t,i}}(\btheta) \Vert_{\bLambda_{T_{t,i}}}
\: .
\end{align*}
We obtain
\begin{align*}
\frac{1}{2}\Vert \hat{\btheta}_t - \btheta'_{\istar,\bT_t}(\hat{\btheta}_t) \Vert_{\bLambda_{\bT_t}}^2
&\ge \frac{1}{2} \left(\Vert \btheta - \btheta'_{\istar,\bT_t}(\hat{\btheta}_t) \Vert_{\bLambda_{\bT_t}} -\Vert \hat{\btheta}_t -\btheta \Vert_{\bLambda_{\bT_t}} \right)^2
\\
&\ge \frac{1}{2}\Vert \btheta - \btheta'_{\istar,\bT_t}(\hat{\btheta}_t) \Vert_{\bLambda_{\bT_t}}^2
	-  \Vert \hat{\btheta}_t -\btheta \Vert_{\bLambda_{\bT_t}} \Vert \btheta - \btheta'_{\istar,\bT_t}(\hat{\btheta}_t) \Vert_{\bLambda_{\bT_t}}
\,.
\end{align*}
By definition of the event $\cE_t$ we know that $\frac{1}{2}\Vert \hat{\btheta}_t -\btheta \Vert_{\bLambda_{\bT_t}}^2 \leq h(t)$ where $h(t)$ is of order $O(\log(t))$. Thus we get
\begin{align*}
\frac{1}{2}\Vert \hat{\btheta}_t - \btheta'_{\istar,\bT_t}(\hat{\btheta}_t) \Vert_{\bLambda_{\bT_t}}^2 &\ge \frac{1}{2} \Vert \btheta - \btheta'_{\istar,\bT_t}(\hat{\btheta}_t) \Vert_{\bLambda_{\bT_t}}^2 - \sqrt{4 h(t) \frac{1}{2}\Vert \btheta - \btheta'_{\istar,\bT_t}(\hat{\btheta}_t) \Vert_{\bLambda_{\bT_t}}^2}\,,
\end{align*}
which leads to, using Lemma~\ref{lem:inq_revert_sqrt},
\begin{equation}
\label{eq:to_theta_nc}
d_{t,\delta} + \sqrt{4 h(t) d_{t,\delta}} +4h(t) \geq \frac{1}{2} \Vert \btheta - \btheta'_{\istar,\bT_t}(\hat{\btheta}_t) \Vert_{\bLambda_{\bT_t}}^2 \,.
\end{equation}
We now continue the proof by finding a lower bound for the right hand sum. Using a tracking property from~\cite{degenne2020structure} to state that for all $a$, $- \log(A) \le T_t^{\bx} - W_t^{\bx}\le 1$, we get
\begin{align*}
\frac{1}{2} \Vert \btheta - \btheta'_{\istar,\bT_t}(\hat{\btheta}_t) \Vert_{\bLambda_{\bT_t}}^2
&\ge \frac{1}{2} \Vert \btheta - \btheta'_{\istar,\bT_t}(\hat{\btheta}_t) \Vert_{\bLambda_{W_t}}^2
	- \frac{\log(A)}{2} \sum_{\bx\in\cX} \Vert \btheta - \btheta'_{\istar,\bT_t}(\hat{\btheta}_t) \Vert_{\bx\bx\transpose}^2
\\
&\ge \frac{1}{2} \Vert \btheta - \btheta'_{\istar,\bT_t}(\hat{\btheta}_t) \Vert_{\bLambda_{W_t}}^2
	- \frac{\log(A)}{2} \sqrt{\sum_{\bx\in\cX} T_t^{\bx}\Vert \btheta - \btheta'_{\istar,\bT_t}(\hat{\btheta}_t) \Vert_{\bx\bx\transpose}^2\sum_{a:T_t^\bx\ge 1} \frac{1}{T_t^\bx}   }
\\
&=   \frac{1}{2} \Vert \btheta - \btheta'_{\istar,\bT_t}(\hat{\btheta}_t) \Vert_{\bLambda_{W_t}}^2
	- \frac{\log(A)}{2} \sqrt{\Vert \btheta - \btheta'_{\istar,\bT_t}(\hat{\btheta}_t) \Vert_{\bLambda_{\bT_t}}^2\sum_{a:T_t^\bx\ge 1} \frac{1}{T_t^\bx}   }
\\
&\ge \frac{1}{2} \Vert \btheta - \btheta'_{\istar,\bT_t}(\hat{\btheta}_t) \Vert_{\bLambda_{W_t}}^2
	-\frac{\log(A)}{2} \sqrt{ A \Vert \btheta - \btheta'_{\istar,\bT_t}(\hat{\btheta}_t) \Vert_{\bLambda_{\bT_t}}^2  }\,.
\end{align*}
%\todo[inline]{TODO: it seems that we introduce a $\sqrt{t}$ factor that should not be there when the $N$ are introduced and then lower bounded by 1.}
Combining the last inequality with \eqref{eq:to_theta_nc} yields
\begin{align*}
    &d_{t,\delta} + \sqrt{4 h(t) d_{t,\delta}} +4h(t)+\frac{\log(A)}{2} \sqrt{2 A}\sqrt{d_{t,\delta} + \sqrt{4 h(t) d_{t,\delta}} +4h(t)}\\
    &\geq \frac{1}{2} \Vert \btheta - \btheta'_{\istar,\bT_t}(\hat{\btheta}_t) \Vert_{\bLambda_{W_t}}^2\,.
\end{align*}
Some simplifications, using the fact that $h(t)\geq 1 $, give us
\begin{equation}
  \label{eq:to_tW_nc}
  d_{t,\delta}+6A\left( \sqrt{h(t)d_{t,\delta}}+2h(t)\right)
  \geq  \frac{1}{2} \Vert \btheta - \btheta'_{\istar,\bT_t}(\hat{\btheta}_t) \Vert_{\bLambda_{W_t}}^2\,.
\end{equation}
We now go from $\btheta$ to each $\hat{\btheta}_s$ for $s \le t$ in the right hand term of the inequality above
\begin{align}
\frac{1}{2}\Vert \btheta - \btheta'_{\istar,\bT_t}(\hat{\btheta}_t) \Vert_{\bLambda_{W_t}}^2
&=   \frac{1}{2} \sum_{s=1}^t  \Vert \btheta - \btheta'_{\istar,\bT_t}(\hat{\btheta}_t) \Vert_{\bLambda_{w_s}}^2
\nonumber\\
&\ge \frac{1}{2} \sum_{s=1}^t \left(\Vert \hat{\btheta}_{s-1} - \btheta'_{\istar,\bT_t}(\hat{\btheta}_t)\Vert_{\bLambda_{w_s}}^2 - 2\Vert \btheta - \hat{\btheta}_{s-1} \Vert_{\bLambda_{w_s}} \Vert \hat{\btheta}_{s-1} - \btheta'_{\istar,\bT_t}(\hat{\btheta}_t) \Vert_{\bLambda_{w_s}}\right)
\nonumber\\
&\ge \frac{1}{2} \sum_{s=1}^t \Vert \hat{\btheta}_{s-1} - \btheta'_{\istar,\bT_t}(\hat{\btheta}_t) \Vert_{\bLambda_{w_s}}^2
\nonumber\\
&\ - \sqrt{\sum_{s=1}^t \Vert \btheta - \hat{\btheta}_{s-1} \Vert_{\bLambda_{w_s}}^2 \sum_{s=1}^t\Vert \hat{\btheta}_{s-1} -\btheta'_{\istar,\bT_t}(\hat{\btheta}_t) \Vert_{\bLambda_{w_s}}^2}
\: .\label{eq:tempW_nc}
\end{align}
We need to upper bound the quantity $\sum_{s=1}^t  w_s^{\bx}\Vert \btheta - \hat{\btheta}_{s-1} \Vert_{\bx\bx\transpose}^2$. By definition of the event $\cE_t$ we have
\begin{align*}
  \Vert \btheta - \hat{\btheta}_{s-1} \Vert_{\bx\bx\transpose}^2 &=  \langle \btheta - \hat{\btheta}_{s-1} ,\bx\rangle^2\\
  &\leq\normm{ \btheta - \hat{\btheta}_{s-1}}_{\bLambda_{\bT_{s-1}}+\lambda I_d}^2 \normm{ a}_{(\bLambda_{\bT_{s-1}}+\lambda I_d)^{-1}}^2\\
  &\leq 2 h(t) \normm{\bx}_{(\bLambda_{\bT_{s-1}}+\lambda I_d)^{-1}}^2\,.
\end{align*}
Thus thanks to Lemma~\ref{lem:computation_sum_w_a_N} we get
\begin{align*}
  \sum_{s=1}^t \sum_{\bx\in\cX} w_s^{\bx}\Vert \btheta - \hat{\btheta}_{s-1} \Vert_{\bx\bx\transpose}^2 \leq 2h(t)\sum_{s=1}^t \sum_{\bx\in\cX} \tw_s^{\bx} \normm{ \bx}_{(\bLambda_{\bT_{s-1}}+\lambda I_d)^{-1}}^2 \leq 2h(t)g(t)\,.
\end{align*}
Going back to \eqref{eq:tempW_nc} in combination with \eqref{eq:to_tW_nc} and Lemma~\ref{lem:inq_revert_sqrt} leads to
\begin{align}
\label{eq:to_hteta_nc}
d_{t,\delta} + 20 A\left(\sqrt{h(t)g(t) d_{t,\delta}}+ 2h(t)g(t)\right)   \geq
\frac{1}{2}\sum_{s=1}^t \Vert \hat{\btheta}_{s-1} - \btheta'_{\istar,\bT_t}(\hat{\btheta}_t)\Vert_{\bLambda_{\tw_s}}^2\,.
\end{align}
\end{proof}


Lemma~\ref{lem:nc_proof_to_online_formulation} introduces a sum of gains/losses on which our algorithms for pulling and for Nature interact.
By definition of the best response $\tbtheta_s^i = \inf_{\btheta' \in \neg i} \Vert \hat{\btheta}_{s-1} - \btheta' \Vert_{\tw_s^i}^2$, we have
\begin{align}
\frac{1}{2}\sum_{s=1}^t  \Vert \hat{\btheta}_{s-1} - \btheta'_{\istar,\bT_t}(\hat{\btheta}_t)\Vert_{\bLambda_{\tw_s}}^2
&\ge \frac{1}{2} \inf_{\btheta' \in \neg \istar} \sum_s \Vert \hat{\btheta}_{s-1} - \btheta'\Vert_{\bLambda_{w_s^{\istar}}}^2
\nonumber\\
&\geq \frac{1}{2}\sum_{s=1}^t \inf_{\btheta' \in \neg \istar} \Vert \hat{\btheta}_{s-1} - \btheta'\Vert_{\bLambda_{w_s^{\istar}}}^2
\nonumber\\
&= \frac{1}{2}\sum_{s=1}^t \sum_{\bx\in\cX} w_s^{\bx,\istar}\Vert \hat{\btheta}_{s-1} - \tbtheta_s^{\istar}\Vert_{\bx\bx\transpose}^2\label{eq:only_istar}
\end{align}
Note that our algorithm computes $\tbtheta_s^{\istar}$ only when $w_s^{\istar} \neq 0$, i.e. only when $i_s = i^*$.

We now introduce the upper confidence bounds
\[
    U_s^{\bx,i} = \min\!\!\left(\max_\pm\! \left( \langle \hbtheta_{s-1} - \tbtheta^{i}_s), a\rangle \pm \sqrt{2 h(t)} \normm{\bx}_{(\bLambda_{T_s}+\lambda I_d)^{-1} } \right)^2,4L^2M^2\right)\,.
\]

\begin{lemma}
The upper confidence bounds are such that, under $\mathcal E_t$,
\begin{align*}
    \frac{1}{2}\sum_{s=1}^t \sum_{\bx\in\cX} w_s^{\bx,\istar}\Vert \hat{\btheta}_{s-1} - \tbtheta_s^{\istar}\Vert_{\bx\bx\transpose}^2\label{eq:only_istar}
    &\ge \frac{1}{2}\sum_{s=1}^t\sum_{\bx\in\cX} w_s^{\bx,\istar}U_s^{\bx,\istar} - h(t)g(t)\\ 
    &-2\sqrt{ h(t) g(t)}  \sqrt{\frac{1}{2}\sum_{s=1}^t \sum_{\bx\in\cX} w_s^{\bx,\istar}\Vert \hbtheta_{s-1} - \tbtheta_s^{\istar} \Vert_{\bx\bx\transpose}^2}
\end{align*}
\end{lemma}
\begin{proof}
\begin{align*}
U_s^{\bx,i} -\Vert \hbtheta_{s-1} - \tbtheta_s^i\Vert_{\bx\bx\transpose}^2
&\leq   \max_\pm \left( \langle \hbtheta_{s-1} - \btheta',\bx\rangle \pm \sqrt{2 h(t)} \normm{\bx}_{(\bLambda_{\bT_{s-1}}+ \lambda I_d)^{-1}} \right)^2-\Vert \hbtheta_{s-1} - \tbtheta_s^i\Vert_{\bx\bx\transpose}^2\\
&\leq  2h(t)\normm{\bx}^2_{(\bLambda_{\bT_{s-1}}+ \lambda I_d)^{-1}} + 2\sqrt{2 h(t)} \normm{\bx}_{(\bLambda_{\bT_{s-1}}+ \lambda I_d)^{-1}}| \langle \hbtheta_{s-1} - \btheta',\bx\rangle|\,.\\
\end{align*}
Hence summing over times and using the Cauchy-Schwarz inequality we obtain
\begin{align*}
&\frac{1}{2}\sum_{s=1}^t\sum_{\bx\in\cX} w_s^{\bx,\istar}\left(U_s^{\bx,\istar} -\Vert \hat{\btheta}_{s-1} - (\btheta')_s^{\istar}\Vert_{\bx\bx\transpose}^2\right)
\\
&\le \sum_{s=1}^t \sum_{\bx\in\cX} w_s^{\bx,\istar}h(t)\normm{\bx}^2_{(\bLambda_{\bT_{s-1}}+ \lambda I_d)^{-1}} +w_s^{\bx,\istar} \sqrt{2 h(t)} \normm{\bx}_{(\bLambda_{\bT_{s-1}}+ \lambda I_d)^{-1}}| \langle \hbtheta_{s-1} - \btheta',\bx\rangle|
\\
&\le  h(t) \sum_{\bx\in\cX} \sum_{s=1}^t w_s^{\bx,\istar}\normm{\bx}^2_{(\bLambda_{\bT_{s-1}}+ \lambda I_d)^{-1}}\\
&+ \sqrt{2 h(t)} \sqrt{\sum_{\bx\in\cX} \sum_{s=1}^t w_s^{\bx,\istar}\normm{\bx}^2_{(\bLambda_{\bT_{s-1}}+ \lambda I_d)^{-1}}}  \sqrt{\sum_{s=1}^t \sum_{\bx\in\cX} w_s^{\bx,\istar}\Vert \hbtheta_{s-1} - \tbtheta_s^{\istar} \Vert_{\bx\bx\transpose}^2} \\
&\leq h(t)g(t) +2\sqrt{ h(t) g(t)}  \sqrt{\frac{1}{2}\sum_{s=1}^t \sum_{\bx\in\cX} w_s^{\bx,\istar}\Vert \hbtheta_{s-1} - \tbtheta_s^{\istar} \Vert_{\bx\bx\transpose}^2}\,,
% &\le 2 C_t \sum_s \sum_{i,\bx} w_s^{i,\bx} \bx\transpose \bLambda_{T_s^i}^{-1}a + 2\sqrt{2 C_t}\sqrt{\sum_s \sum_{i,\bx} w_s^{i,\bx}\bx\transpose \bLambda_{T_s^i}^{-1}a }\sqrt{\sum_s \sum_{i,\bx} w_s^{i,\bx}\Vert \hat{\btheta}_{s-1} - \btheta'_{s,i}\Vert_{\bx\bx\transpose}^2}
\end{align*}
where in the last inequality we used Lemma~\ref{lem:computation_sum_w_a_N}.
\end{proof}

Thus combining the previous inequality with \eqref{eq:only_istar} and Lemma~\ref{lem:nc_proof_to_online_formulation} yields, with some simplifications,
\begin{equation}
\label{eq:to_UCB}
d_{t,\delta} + 40 A\left(\sqrt{h(t)g(t) d_{t,\delta}}+ 2h(t)g(t)\right) \geq \frac{1}{2}\sum_{s=1}^t\sum_{\bx\in\cX} w_s^{\bx,\istar}U_s^{\bx,\istar}\,.
\end{equation}
Now we control the regret of the learner $\cL_w^{\istar}$, thanks to the bound for \AH, see Lemma~\ref{lemma:lgc.adahedge}, we have
\[
\sup_{w\in\Sigma_K}\frac{1}{2}\sum_{s=1}^t\ind_{\{i_t = \istar\}}\sum_{\bx\in\cX} w^{\bx}U_s^{\bx,\istar} -\frac{1}{2}\sum_{s=1}^t\sum_{\bx\in\cX} w_s^{\bx,\istar}U_s^{\bx,\istar} \leq C'\sqrt{T_{t,i}}\leq C'\sqrt{t}\,.
\]
Then using this inequality in combination with the fact that the losses are optimistic we obtain
\begin{align*}
  d_{t,\delta} + 40 A\left(\sqrt{h(t)g(t) d_{t,\delta}}+ 2h(t)g(t)\right) +C'\sqrt{t}
  &\geq \sup_{w\in\Sigma_K}\frac{1}{2}\sum_{s=1}^t\ind_{\{i_s = \istar\}}\sum_{\bx\in\cX} w^{\bx}U_s^{\bx,\istar}
  \\
  &\geq \sup_{w\in\Sigma_K}\frac{1}{2}\sum_{s=1}^t\ind_{\{i_s = \istar\}}\sum_{\bx\in\cX} w^{\bx} \normm{\btheta -(\btheta'_s)^{\istar}}^2_{\bx\bx\transpose}
  \\
  &= T^{\istar}_t \sup_{w\in\Sigma_K}\frac{1}{T^{i^*}_t}\sum_{s=1}^t\ind_{\{i_s = \istar\}}\frac{1}{2}\normm{\btheta -(\btheta')_s^{\istar}}^2_{\bLambda_{w}}
  \end{align*}
Now remark that $\frac{1}{T^{i^\star}_t}\sum_{s=1}^t\ind_{\{i_s = \istar\}}\frac{1}{2}\normm{\btheta -(\btheta')_s^{\istar}}^2_{\bLambda_{w}}$ is the expectation under some distribution of $\frac{1}{2}\normm{\btheta -(\btheta')_s^{\istar}}^2_{\bLambda_{w}}$ .
\begin{align*}
  d_{t,\delta} + 40 A\left(\sqrt{h(t)g(t) d_{t,\delta}}+ 2h(t)g(t)\right) +C'\sqrt{t}
  &\geq T^{\istar}_t \inf_{q\in\cP(\neg \istar)} \sup_{w\in\Sigma_K}\frac{1}{2}\E_{\btheta'\sim q}\normm{\btheta -\btheta'}^2_{\bLambda_{w}}\\
 &=T^{\istar}_t \Tstar(\btheta)^{-1}\,,
\end{align*}
where in the last line we use the theorem of Sion, see...%\todo{is that equality not proven somewhere else in the paper?}. 
Note that the last inequality holds also if $T_{t,\istar} = 0$. It remains to show that $T^{\istar}_t = t- O(\sqrt{t})$.

\subsection{When $i_s \neq \istar$.}

\begin{theorem}
For $i\in\cI$ and $t\in \mathbb{N}$, let $T_{t,i} = \sum_{s=1}^t \mathbb{I}\{i_s=i\}$. Then under event $\mathcal E_t$,
\begin{align*}
T_t^*
\ge t - \sqrt{t} - \frac{16}{\Delta_{\min}^2}\left((I-1)C'\sqrt{t} + (1 + \sqrt{I-1})^2 h(t)g(t)\right)
\: .
\end{align*}
\end{theorem}

Since $\btheta \in \neg i$ for all $i\neq i^*$, under $\mathcal E_t$%\todo{refer to where the first inequality is proven},
\begin{align*}
h(t)g(t)
\ge \sum_{s=1}^t \sum_{\bx\in\cX} w_s^\bx \frac{1}{2}\Vert \btheta - \hat{\btheta}_{s-1} \Vert_{\bx\bx\transpose}^2
&\ge \sum_{s\le t, i_s\neq i^*} \sum_{\bx\in\cX} w_s^\bx \frac{1}{2}\Vert \btheta - \hat{\btheta}_{s-1} \Vert_{\bx\bx\transpose}^2
\\
&\ge \sum_{j \neq i^*} \inf_{\btheta'\in \neg j} \sum_{s = 1}^t \sum_{\bx\in\cX} w_s^{j,\bx} \frac{1}{2}\Vert \btheta' - \hat{\btheta}_{s-1} \Vert_{\bx\bx\transpose}^2
\: .
\end{align*}

As previously done for $i^*$, we obtain for all $j\neq i^*$,
\begin{align*}
\inf_{\btheta'\in \neg j} \sum_{s = 1}^t \sum_{\bx} w_s^{j,\bx} \frac{1}{2}\Vert \btheta' - \hat{\btheta}_{s-1} \Vert_{\bx\bx\transpose}^2
\ge  \left(\sqrt{\frac{1}{2}\max_{\bx\in\cX} \sum_{s=1}^t \ind_{\{i_s=j\}} U_s^\bx - C'\sqrt{t}} - \sqrt{h(t)g(t)}\right)^2
\: .
\end{align*}

We show that the sum on the right is proportional to its number of terms $n = t - T_t^*$, then use that the sum on the left is $\mathcal O(\sqrt{t})$. We obtain that $n = \mathcal O(\sqrt{t})$.

\begin{lemma}
If the event $\mathcal E_t$ holds, then for all $s\le t$, if $i^*(\hbtheta_s) \neq i^*(\btheta)$ then there exists an arm $\bx\in\cX$ such that
\begin{align*}
U_s^\bx \ge 2 h(s) \bx\transpose \bLambda_{T_s}^{-1}\bx \ge \Delta_{\min}^2/4 \: .
\end{align*}
\end{lemma}

\begin{proof}
If $i^*(\hbtheta_s) \neq i^*(\btheta)$, then there exists an arm $\bx\in\cX$ such that
\begin{align*}
\hbtheta_s\transpose(\bx - \bx^\star(\btheta)) \ge 0
\Rightarrow & (\hbtheta_s - \btheta)\transpose (\bx - \bx^\star(\btheta)) \ge \Delta_{\min}
\\
\Rightarrow & | (\hbtheta_s - \btheta)\transpose \bx | + | (\hbtheta_s - \btheta)\transpose \bx^\star(\btheta) | \ge \Delta_{\min}
\end{align*}
Hence either 
\[
    | (\hbtheta_s - \btheta)\transpose \bx | \ge \frac{\Delta_{\min}}{2}\,,
\]
or
\[
    | (\hbtheta_s - \btheta)\transpose \bx^\star(\btheta) | \ge \frac{\Delta_{\min}}{2}\,.
\]
By consequence, there exists an arm $\bx'$ such that 
\[
    | (\hbtheta_s - \btheta)\transpose \bx' | \ge \frac{\Delta_{\min}}{2}\,.
\]

With the Cauchy-Schwarz inequality, there exists $\bx\in\cX$ such that
\[
    \frac{\Delta_{\min}}{2} \le \sqrt{\Vert \hbtheta_s - \btheta \Vert^2_{\bLambda_{T_s}} \bx\transpose \bLambda_{T_s}^{-1}\bx}\,.
\]
Under the event $\mathcal E_t$ we obtain 
\[
    \frac{\Delta_{\min}}{2} \le \sqrt{2 h(s) \bx\transpose \bLambda_{T_s}^{-1}a} \le \sqrt{U_s^\bx}\,.
\]
\end{proof}

\begin{lemma}
If we have 
\[
    2h(t)\bx\transpose\bLambda_{\bT_t}^{-1}\bx \ge x\,,
\]
then the following holds
\[
    \sum_{s\le t} U_s^\bx \ge x \sum_{s\le t} h(s)/h(t)\,.
\]
\end{lemma}

For $i\neq i^*$, let $t'= \max\{s\le t, i_s = i\}$. Let $a'$ be an arm such that $2h(t')\bx\transpose \bLambda_{N_{t'}}^{-1}a \ge \Delta_{\min}^2/4$. Then
\begin{align*}
\max_{\bx\in \cX}\sum_{s\le t, i_s=i} U_s^\bx
\ge \sum_{s\le t, i_s=i} U_s^{\bx'}
&\ge \frac{\Delta_{\min}^2}{4} \sum_{s\le t, i_s=i} h(s)/h(t)
\\
&\ge \frac{\Delta_{\min}^2}{4} \sum_{\sqrt{t} \le s\le t, i_s=i} h(s)/h(t)
\\
&\ge \frac{\Delta_{\min}^2}{4} \sum_{\sqrt{t} \le s\le t, i_s=i} \frac{1}{2}
\\
&= \frac{\Delta_{\min}^2}{8} (T_{t,i} - N_{\sqrt{t}}^i)
\end{align*}
%\todo{check the lower bound by 1/2}

We get that $\sum_{i\neq i^*}\max_{\bx\in \cX}\sum_{s\le t, i_s=i} U_s^\bx \ge \frac{\Delta_{\min}^2}{8} (t - T_t^* - \sqrt{t})$ .

\begin{align*}
    h(t)g(t) &\ge \sum_{j\neq i^*} \left(\sqrt{\frac{1}{2}\max_{\bx\in \mathcal A} \sum_{s=1}^t \ind_{\{i_s=j\}} U_s^\bx - C'\sqrt{t}} - \sqrt{h(t)g(t)}\right)^2\\
    &\ge \sum_{j\neq i^*} \left(\sqrt{\frac{\Delta_{\min}^2}{16} (T_{t,j} - N_{\sqrt{t}}^j) - C'\sqrt{t}} - \sqrt{h(t)g(t)}\right)^2\\
    &= \frac{\Delta_{\min}^2}{16} (t - T_t^* - \sqrt{t} + N_{\sqrt{t}}^*) - (I-1)C'\sqrt{t}\\
    &- 2\sqrt{h(t)g(t)}\sum_{j\neq i^*}\sqrt{\frac{\Delta_{\min}^2}{16} (T_{t,j} - N_{\sqrt{t}}^j) - C'\sqrt{t}} + (I-1)h(t)g(t)\\
    &\ge \frac{\Delta_{\min}^2}{16} (t - T_t^* - \sqrt{t} + N_{\sqrt{t}}^*) - (I-1)C'\sqrt{t}\\
    &- 2\sqrt{(I-1) h(t)g(t)}\sqrt{\sum_{j\neq i^*}(\frac{\Delta_{\min}^2}{16} (T_{t,j} - N_{\sqrt{t}}^j) - C'\sqrt{t})} + (I-1)h(t)g(t)\\
    &= \frac{\Delta_{\min}^2}{16} (t - T_t^* - \sqrt{t} + N_{\sqrt{t}}^*) - (I-1)C'\sqrt{t}\\
    &- 2\sqrt{(I-1) h(t)g(t)}\sqrt{\frac{\Delta_{\min}^2}{16} (t - T_t^* - \sqrt{t} + N_{\sqrt{t}}^*) - (I-1)C'\sqrt{t})} + (I-1)h(t)g(t)\\
    &= \left( \sqrt{\frac{\Delta_{\min}^2}{16} (t - T_t^* - \sqrt{t} + N_{\sqrt{t}}^*) - (I-1)C'\sqrt{t})} - \sqrt{(I-1) h(t)g(t)} \right)^2\,.
\end{align*}

\begin{align*}
    &\frac{\Delta_{\min}^2}{16} (t - T_t^* - \sqrt{t} + N_{\sqrt{t}}^*) - (I-1)C'\sqrt{t} \le (1 + \sqrt{I-1})^2 h(t)g(t)\\
    \Rightarrow
    &t - T_t^*
    \le \sqrt{t} + \frac{16}{\Delta_{\min}^2}\left((I-1)C'\sqrt{t} + (1 + \sqrt{I-1})^2 h(t)g(t)\right)\,.
\end{align*}